theories/Classes/Relations.v
@@ -1,0 +1,569 @@
+(* -*- coq-prog-args: ("-emacs-U" "-nois") -*- *)
+(************************************************************************)
+(*  v      *   The Coq Proof Assistant  /  The Coq Development Team     *)
+(* <O___,, * CNRS-Ecole Polytechnique-INRIA Futurs-Universite Paris Sud *)
+(*   \VV/  **************************************************************)
+(*    //   *      This file is distributed under the terms of the       *)
+(*         *       GNU Lesser General Public License Version 2.1        *)
+(************************************************************************)
+
+(* Typeclass-based setoids, tactics and standard instances.
+   TODO: explain clrewrite, clsubstitute and so on.
+ 
+   Author: Matthieu Sozeau
+   Institution: LRI, CNRS UMR 8623 - UniversitÃcopyright Paris Sud
+   91405 Orsay, France *)
+
+(* $Id: FSetAVL_prog.v 616 2007-08-08 12:28:10Z msozeau $ *)
+
+Require Import Coq.Program.Program.
+Require Import Coq.Classes.Init.
+
+Set Implicit Arguments.
+Unset Strict Implicit.
+
+Definition relationT A := A -> A -> Type.
+Definition relation A := A -> A -> Prop.
+
+Definition inverse A (R : relation A) : relation A := flip R.
+
+Lemma inverse_inverse : forall A (R : relation A), inverse (inverse R) = R.
+Proof. intros ; unfold inverse. apply (flip_flip R). Qed.
+
+Definition complementT A (R : relationT A) := fun x y => ! R x y.
+
+Definition complement A (R : relation A) := fun x y => ~ R x y.
+
+(** These are convertible. *)
+
+Lemma complementT_flip : forall A (R : relationT A), complementT (flip R) = flip (complementT R).
+Proof. reflexivity. Qed.
+
+Lemma complement_inverse : forall A (R : relation A), complement (inverse R) = inverse (complement R).
+Proof. reflexivity. Qed.
+
+(** We rebind relations in separate classes to be able to overload each proof. *)
+
+Class Reflexive A (R : relationT A) :=
+  reflexive : forall x, R x x.
+
+Class Irreflexive A (R : relationT A) := 
+  irreflexive : forall x, R x x -> False.
+
+Class Symmetric A (R : relationT A) := 
+  symmetric : forall x y, R x y -> R y x.
+
+Class Asymmetric A (R : relationT A) := 
+  asymmetric : forall x y, R x y -> R y x -> False.
+
+Class Transitive A (R : relationT A) := 
+  transitive : forall x y z, R x y -> R y z -> R x z.
+
+Implicit Arguments Reflexive [A].
+Implicit Arguments Irreflexive [A].
+Implicit Arguments Symmetric [A].
+Implicit Arguments Asymmetric [A].
+Implicit Arguments Transitive [A].
+
+Hint Resolve @irreflexive : ord.
+
+(** We can already dualize all these properties. *)
+
+Program Instance [ Reflexive A R ] => flip_reflexive : Reflexive A (flip R) :=
+  reflexive := reflexive (R:=R).
+
+Program Instance [ Irreflexive A R ] => flip_irreflexive : Irreflexive A (flip R) :=
+  irreflexive := irreflexive (R:=R).
+
+Program Instance [ Symmetric A R ] => flip_symmetric : Symmetric A (flip R).
+
+  Solve Obligations using unfold flip ; program_simpl ; eapply symmetric ; eauto.
+
+Program Instance [ Asymmetric A R ] => flip_asymmetric : Asymmetric A (flip R).
+  
+  Solve Obligations using program_simpl ; unfold flip in * ; intros ; eapply asymmetric ; eauto.
+
+Program Instance [ Transitive A R ] => flip_transitive : Transitive A (flip R).
+
+  Solve Obligations using unfold flip ; program_simpl ; eapply transitive ; eauto.
+
+(** Have to do it again for Prop. *)
+
+Program Instance [ Reflexive A (R : relation A) ] => inverse_reflexive : Reflexive A (inverse R) :=
+  reflexive := reflexive (R:=R).
+
+Program Instance [ Irreflexive A (R : relation A) ] => inverse_irreflexive : Irreflexive A (inverse R) :=
+  irreflexive := irreflexive (R:=R).
+
+Program Instance [ Symmetric A (R : relation A) ] => inverse_symmetric : Symmetric A (inverse R).
+
+  Solve Obligations using unfold inverse, flip ; program_simpl ; eapply symmetric ; eauto.
+
+Program Instance [ Asymmetric A (R : relation A) ] => inverse_asymmetric : Asymmetric A (inverse R).
+  
+  Solve Obligations using program_simpl ; unfold inverse, flip in * ; intros ; eapply asymmetric ; eauto.
+
+Program Instance [ Transitive A (R : relation A) ] => inverse_transitive : Transitive A (inverse R).
+
+  Solve Obligations using unfold inverse, flip ; program_simpl ; eapply transitive ; eauto.
+
+Program Instance [ Reflexive A (R : relation A) ] => 
+  reflexive_complement_irreflexive : Irreflexive A (complement R).
+
+  Next Obligation. 
+  Proof. 
+    unfold complement in * ; intros.
+    apply H.
+    apply reflexive.
+  Qed.
+
+Program Instance [ Irreflexive A (R : relation A) ] => 
+  irreflexive_complement_reflexive : Reflexive A (complement R).
+
+  Next Obligation. 
+  Proof. 
+    unfold complement in * ; intros.
+    red ; intros.
+    apply (irreflexive H).
+  Qed.
+
+Program Instance [ Symmetric A (R : relation A) ] => complement_symmetric : Symmetric A (complement R).
+
+  Next Obligation.
+  Proof.
+    unfold complement in *.
+    red ; intros H'.
+    apply (H (symmetric H')).
+  Qed.
+
+(** Tactics to solve goals. Each tactic comes in two flavors:
+   - a tactic to immediately solve a goal without user intervention
+   - a tactic taking input from the user to make progress on a goal *)
+
+Definition relate A (R : relationT A) : relationT A := R.
+
+Ltac relationify_relation R R' :=
+  match goal with
+    | [ H : context [ R ?x ?y ] |- _ ] => change (R x y) with (R' x y) in H
+    | [ |- context [ R ?x ?y ] ] => change (R x y) with (R' x y)
+  end.
+
+Ltac relationify R :=
+  set (R' := relate R) ; progress (repeat (relationify_relation R R')).
+
+Ltac relation_refl :=
+  match goal with
+    | [ |- ?R ?X ?X ] => apply (reflexive (R:=R) X)
+    | [ H : ?R ?X ?X |- _ ] => apply (irreflexive (R:=R) H)
+
+    | [ |- ?R ?A ?X ?X ] => apply (reflexive (R:=R A) X)
+    | [ H : ?R ?A ?X ?X |- _ ] => apply (irreflexive (R:=R A) H)
+
+    | [ |- ?R ?A ?B ?X ?X ] => apply (reflexive (R:=R A B) X)
+    | [ H : ?R ?A ?B ?X ?X |- _ ] => apply (irreflexive (R:=R A B) H)
+
+    | [ |- ?R ?A ?B ?C ?X ?X ] => apply (reflexive (R:=R A B C) X)
+    | [ H : ?R ?A ?B ?C ?X ?X |- _ ] => apply (irreflexive (R:=R A B C) H)
+
+    | [ |- ?R ?A ?B ?C ?D ?X ?X ] => apply (reflexive (R:=R A B C D) X)
+    | [ H : ?R ?A ?B ?C ?D ?X ?X |- _ ] => apply (irreflexive (R:=R A B C D) H)
+  end.
+
+Ltac refl := relation_refl.
+
+Ltac relation_sym := 
+  match goal with
+    | [ H : ?R ?X ?Y |- ?R ?Y ?X ] => apply (symmetric (R:=R) (x:=X) (y:=Y) H)
+
+    | [ H : ?R ?A ?X ?Y |- ?R ?A ?Y ?X ] => apply (symmetric (R:=R A) (x:=X) (y:=Y) H)
+
+    | [ H : ?R ?A ?B ?X ?Y |- ?R ?A ?B ?Y ?X ] => apply (symmetric (R:=R A B) (x:=X) (y:=Y) H)
+
+    | [ H : ?R ?A ?B ?C ?X ?Y |- ?R ?A ?B ?C ?Y ?X ] => apply (symmetric (R:=R A B C) (x:=X) (y:=Y) H)
+
+    | [ H : ?R ?A ?B ?C ?D ?X ?Y |- ?R ?A ?B ?C ?D ?Y ?X ] => apply (symmetric (R:=R A B C D) (x:=X) (y:=Y) H)
+
+  end.
+
+Ltac relation_symmetric := 
+  match goal with
+    | [ |- ?R ?Y ?X ] => apply (symmetric (R:=R) (x:=X) (y:=Y))
+
+    | [ |- ?R ?A ?Y ?X ] => apply (symmetric (R:=R A) (x:=X) (y:=Y))
+
+    | [ |- ?R ?A ?B ?Y ?X ] => apply (symmetric (R:=R A B) (x:=X) (y:=Y))
+
+    | [ |- ?R ?A ?B ?C ?Y ?X ] => apply (symmetric (R:=R A B C) (x:=X) (y:=Y))
+
+    | [ |- ?R ?A ?B ?C ?D ?Y ?X ] => apply (symmetric (R:=R A B C D) (x:=X) (y:=Y))
+  end.
+
+Ltac sym := relation_symmetric.
+
+Ltac relation_trans := 
+  match goal with
+    | [ H : ?R ?X ?Y, H' : ?R ?Y ?Z |- ?R ?X ?Z ] => 
+      apply (transitive (R:=R) (x:=X) (y:=Y) (z:=Z) H H')
+
+    | [ H : ?R ?A ?X ?Y, H' : ?R ?A ?Y ?Z |- ?R ?A ?X ?Z ] => 
+      apply (transitive (R:=R A) (x:=X) (y:=Y) (z:=Z) H H')
+
+    | [ H : ?R ?A ?B ?X ?Y, H' : ?R ?A ?B ?Y ?Z |- ?R ?A ?B ?X ?Z ] => 
+      apply (transitive (R:=R A B) (x:=X) (y:=Y) (z:=Z) H H')
+
+    | [ H : ?R ?A ?B ?C ?X ?Y, H' : ?R ?A ?B ?C ?Y ?Z |- ?R ?A ?B ?C ?X ?Z ] => 
+      apply (transitive (R:=R A B C) (x:=X) (y:=Y) (z:=Z) H H')
+
+    | [ H : ?R ?A ?B ?C ?D ?X ?Y, H' : ?R ?A ?B ?C ?D ?Y ?Z |- ?R ?A ?B ?C ?D ?X ?Z ] => 
+      apply (transitive (R:=R A B C D) (x:=X) (y:=Y) (z:=Z) H H')
+  end.
+
+Ltac relation_transitive Y := 
+  match goal with
+    | [ |- ?R ?X ?Z ] => 
+      apply (transitive (R:=R) (x:=X) (y:=Y) (z:=Z))
+
+    | [ |- ?R ?A ?X ?Z ] => 
+      apply (transitive (R:=R A) (x:=X) (y:=Y) (z:=Z))
+
+    | [ |- ?R ?A ?B ?X ?Z ] => 
+      apply (transitive (R:=R A B) (x:=X) (y:=Y) (z:=Z))
+
+    | [ |- ?R ?A ?B ?C ?X ?Z ] => 
+      apply (transitive (R:=R A B C) (x:=X) (y:=Y) (z:=Z))
+
+    | [ |- ?R ?A ?B ?C ?D ?X ?Z ] => 
+      apply (transitive (R:=R A B C D) (x:=X) (y:=Y) (z:=Z))
+  end.
+
+Ltac trans Y := relation_transitive Y.
+
+(** To immediatly solve a goal on setoid equality. *)
+
+Ltac relation_tac := relation_refl || relation_sym || relation_trans.
+
+(** * Morphisms.
+
+   We now turn to the definition of [Morphism] and declare standard instances. 
+   These will be used by the [clrewrite] tactic later. *)
+
+(** Respectful morphisms. *)
+
+Definition respectful_depT (A : Type) (R : relationT A) 
+  (B : A -> Type) (R' : forall x y, B x -> B y -> Type) : relationT (forall x : A, B x) := 
+  fun f g => forall x y : A, R x y -> R' x y (f x) (g y).
+
+Definition respectfulT A (eqa : relationT A) B (eqb : relationT B) : relationT (A -> B) :=
+  Eval compute in (respectful_depT eqa (fun _ _ => eqb)).
+
+Definition respectful A (R : relation A) B (R' : relation B) : relation (A -> B) :=
+  fun f g => forall x y : A, R x y -> R' (f x) (g y).
+
+(** Notations reminiscent of the old syntax for declaring morphisms.
+   We use three + or - for type morphisms, and two for [Prop] ones.
+   *)
+
+Notation " R +++> R' " := (@respectfulT _ R _ R') (right associativity, at level 20).
+Notation " R ---> R' " := (@respectfulT _ (flip R) _ R') (right associativity, at level 20).
+
+Notation " R ++> R' " := (@respectful _ R _ R') (right associativity, at level 20).
+Notation " R --> R' " := (@respectful _ (inverse R) _ R') (right associativity, at level 20).
+
+(** A morphism on a relation [R] is an object respecting the relation (in its kernel). 
+   The relation [R] will be instantiated by [respectful] and [A] by an arrow type 
+   for usual morphisms. *)
+
+Class Morphism A (R : relationT A) (m : A) :=
+  respect : R m m.
+
+Ltac simpl_morphism :=
+  try red ; unfold inverse, flip, impl, arrow ; program_simpl ; try tauto ; 
+    try (red ; intros) ; try ( solve [ intuition ]).
+
+Ltac obligations_tactic ::= simpl_morphism.
+
+(** The arrow is a reflexive and transitive relation on types. *)
+
+Program Instance arrow_refl : ? Reflexive arrow := 
+  reflexive X := id.
+
+Program Instance arrow_trans : ? Transitive arrow := 
+  transitive X Y Z f g := g o f.
+
+(** Can't use the definition [notT] as it gives a to universe inconsistency. *)
+
+Program Instance notT_arrow_morphism : 
+  Morphism (Type -> Type) (arrow ---> arrow) (fun X : Type => X -> False).
+
+(** Isomorphism. *)
+
+Definition iso (A B : Type) := 
+  A -> B * B -> A.
+
+Program Instance iso_refl : ? Reflexive iso.
+Program Instance iso_sym : ? Symmetric iso.
+Program Instance iso_trans : ? Transitive iso.
+
+Program Instance not_iso_morphism : 
+  Morphism (Type -> Type) (iso +++> iso) (fun X : Type => X -> False).
+
+(** Logical implication. *)
+
+Program Instance impl_refl : ? Reflexive impl.
+Program Instance impl_trans : ? Transitive impl.
+
+Program Instance not_impl_morphism :
+  Morphism (Prop -> Prop) (impl --> impl) not.
+
+(** Logical equivalence. *)
+
+Program Instance iff_refl : ? Reflexive iff.
+Program Instance iff_sym : ? Symmetric iff.
+Program Instance iff_trans : ? Transitive iff.
+
+Program Instance not_iff_morphism : 
+  Morphism (Prop -> Prop) (iff ++> iff) not.
+
+(** We make the type implicit, it can be infered from the relations. *)
+
+Implicit Arguments Morphism [A].
+
+(** If you have a morphism from [RA] to [RB] you have a contravariant morphism 
+   from [RA] to [inverse RB]. *)
+
+Program Instance `A` (RA : relation A) `B` (RB : relation B) [ ? Morphism (RA ++> RB) m ] =>
+  morph_impl_co_contra_inverse :
+  ? Morphism (RA --> inverse RB) m.
+
+  Next Obligation.
+  Proof.
+    apply respect.
+    apply H.
+  Qed.
+
+(** Every transitive relation gives rise to a binary morphism on [impl], 
+   contravariant in the first argument, covariant in the second. *)
+
+Program Instance [ Transitive A (R : relation A) ] => 
+  trans_contra_co_morphism : ? Morphism (R --> R ++> impl) R.
+
+  Next Obligation.
+  Proof with auto.
+    trans x...
+    trans x0...
+  Qed.
+
+(** Dually... *)
+
+Program Instance [ Transitive A (R : relation A) ] =>
+  trans_co_contra_inv_impl_morphism : ? Morphism (R ++> R --> inverse impl) R.
+
+  Obligations Tactic := idtac.
+  
+  Next Obligation.
+  Proof with auto.
+    intros.
+    destruct (trans_contra_co_morphism (R:=inverse R)).
+    revert respect0.
+    unfold respectful, inverse, flip in * ; intros.
+    apply respect0 ; auto.
+  Qed.
+
+Obligations Tactic := simpl_morphism.
+
+(** With symmetric relations, variance is no issue ! *)
+
+Program Instance [ Symmetric A (R : relation A) ] B (R' : relation B) 
+  [ Morphism _ (R ++> R') m ] => 
+  sym_contra_morphism : ? Morphism (R --> R') m.
+
+  Next Obligation.
+  Proof with auto.
+    apply respect.
+    sym...
+  Qed.
+
+(** Every symmetric and transitive relation gives rise to an equivariant morphism. *)
+
+Program Instance [ Transitive A (R : relation A), Symmetric A R ] => 
+  trans_sym_morphism : ? Morphism (R ++> R ++> iff) R.
+
+  Next Obligation.
+  Proof with auto.
+    split ; intros.
+    trans x0... trans x... sym...
+  
+    trans y... trans y0... sym...
+  Qed.
+
+(** The complement of a relation conserves its morphisms. *)
+
+Program Instance `A` (RA : relation A) [ ? Morphism (RA ++> RA ++> iff) R ] => 
+  complement_morphism : ? Morphism (RA ++> RA ++> iff) (complement R).
+
+  Next Obligation.
+  Proof.
+    red ; unfold complement ; intros.
+    pose (respect).
+    pose (r x y H).
+    pose (r0 x0 y0 H0).
+    intuition.
+  Qed.
+
+(** The inverse too. *)
+
+Program Instance `A` (RA : relation A) [ ? Morphism (RA ++> RA ++> iff) R ] => 
+  inverse_morphism : ? Morphism (RA ++> RA ++> iff) (inverse R).
+
+  Next Obligation.
+  Proof.
+    unfold inverse ; unfold flip.
+    apply respect ; auto.
+  Qed.
+
+Program Instance [ Transitive A (R : relation A), Symmetric A R ] =>
+  trans_sym_contra_co_inv_impl_morphism : ? Morphism (R --> R ++> inverse impl) R.
+
+  Next Obligation.
+  Proof with auto.
+    trans y...
+    sym...
+    trans y0...
+    sym...
+  Qed.
+
+(** Any binary morphism respecting some relations up to [iff] respects 
+   them up to [impl] in each way. Very important instances as we need [impl]
+   morphisms at the top level when we rewrite. *)
+
+Program Instance `A` (R : relation A) `B` (R' : relation B) 
+  [ ? Morphism (R ++> R' ++> iff) m ] => 
+  iff_impl_binary_morphism : ? Morphism (R ++> R' ++> impl) m.
+
+  Next Obligation.
+  Proof.
+    destruct respect with x y x0 y0 ; auto.
+  Qed.
+
+Program Instance `A` (R : relation A) `B` (R' : relation B)
+  [ ? Morphism (R ++> R' ++> iff) m ] => 
+  iff_inverse_impl_binary_morphism : ? Morphism (R ++> R' ++> inverse impl) m.
+
+  Next Obligation.
+  Proof.
+    destruct respect with x y x0 y0 ; auto.
+  Qed.
+
+(** Standard instances for [iff] and [impl]. *)
+
+(** Logical conjunction. *)
+
+Program Instance and_impl_iff_morphism : ? Morphism (impl ++> iff ++> impl) and.
+
+Program Instance and_iff_impl_morphism : ? Morphism (iff ++> impl ++> impl) and.
+
+Program Instance and_iff_morphism : ? Morphism (iff ++> iff ++> iff) and.
+
+(** Logical disjunction. *)
+
+Program Instance or_impl_iff_morphism : ? Morphism (impl ++> iff ++> impl) or.
+
+Program Instance or_iff_impl_morphism : ? Morphism (iff ++> impl ++> impl) or.
+
+Program Instance or_iff_morphism : ? Morphism (iff ++> iff ++> iff) or.
+
+(** Leibniz equality. *)
+
+Program Instance eq_refl : ? Reflexive (@eq A).
+Program Instance eq_sym : ? Symmetric (@eq A).
+Program Instance eq_trans : ? Transitive (@eq A).
+
+Program Definition eq_morphism A : Morphism (eq ++> eq ++> iff) (eq (A:=A)) :=
+  trans_sym_morphism.
+
+Program Instance `A B` (m : A -> B) => arrow_morphism : ? Morphism (eq ++> eq) m.
+
+(** The [PER] typeclass. *)
+
+Class PER (carrier : Type) (pequiv : relationT carrier) :=
+  per_sym :> Symmetric pequiv ;
+  per_trans :> Transitive pequiv.
+
+(** We can build a PER on the coq function space if we have PERs on the domain and
+   codomain. *)
+
+Program Instance [ PER A (R : relation A), PER B (R' : relation B) ] => 
+  arrow_per : PER (A -> B)
+  (fun f g => forall (x y : A), R x y -> R' (f x) (g y)).
+
+  Next Obligation.
+  Proof with auto.
+    constructor ; intros...
+    assert(R x0 x0) by (trans y0 ; [ auto | sym ; auto ]).
+    trans (y x0)...
+  Qed.
+
+(** The [Equivalence] typeclass. *)
+
+Class Equivalence (carrier : Type) (equiv : relationT carrier) :=
+  equiv_refl :> Reflexive equiv ;
+  equiv_sym :> Symmetric equiv ;
+  equiv_trans :> Transitive equiv.
+
+(** We can now define antisymmetry w.r.t. an equivalence relation on the carrier. *)
+
+Class [ Equivalence A eqA ] => Antisymmetric (R : relationT A) := 
+  antisymmetric : forall x y, R x y -> R y x -> eqA x y.
+
+Program Instance [ eq : Equivalence A eqA, ? Antisymmetric eq R ] => 
+  flip_antisymmetric : ? Antisymmetric eq (flip R).
+
+  Solve Obligations using unfold flip ; program_simpl ; eapply antisymmetric ; eauto.
+
+(** Here we build an equivalence instance for functions which relates respectful ones only. *)
+
+Definition respecting [ Equivalence A (R : relation A), Equivalence B (R' : relation B) ] : Type := 
+  { morph : A -> B | respectful R R' morph morph }.
+
+Ltac obligations_tactic ::= program_simpl.
+
+Program Instance [ Equivalence A (R : relation A), Equivalence B (R' : relation B) ] => 
+  respecting_equiv : Equivalence respecting
+  (fun (f g : respecting) => forall (x y : A), R x y -> R' (`f x) (`g y)).
+
+  Next Obligation.
+  Proof.
+    constructor ; intros.
+    destruct x ; simpl.
+    apply r ; auto.
+  Qed.
+
+  Next Obligation.
+  Proof.
+    constructor ; intros.
+    sym ; apply H.
+    sym ; auto.
+  Qed.
+
+  Next Obligation.
+  Proof.
+    constructor ; intros.
+    trans ((`y) y0).
+    apply H ; auto.
+    apply H0. refl.
+  Qed.
+
+(** Leibinz equality [eq] is an equivalence relation. *)
+
+Program Instance eq_equivalence : Equivalence A eq.
+
+(** Logical equivalence [iff] is an equivalence relation. *)
+
+Program Instance iff_equivalence : Equivalence Prop iff.
+
+(** The following is not definable. *)
+(*
+Program Instance [ sa : Equivalence a R, sb : Equivalence b R' ] => equiv_setoid : 
+  Equivalence (a -> b)
+  (fun f g => forall (x y : a), R x y -> R' (f x) (g y)).
+*)
