theories/Program/Basics.v
@@ -1,0 +1,143 @@
+(* -*- coq-prog-args: ("-emacs-U" "-nois") -*- *)
+(************************************************************************)
+(*  v      *   The Coq Proof Assistant  /  The Coq Development Team     *)
+(* <O___,, * CNRS-Ecole Polytechnique-INRIA Futurs-Universite Paris Sud *)
+(*   \VV/  **************************************************************)
+(*    //   *      This file is distributed under the terms of the       *)
+(*         *       GNU Lesser General Public License Version 2.1        *)
+(************************************************************************)
+
+(* Standard functions and proofs about them.
+ * Author: Matthieu Sozeau
+ * Institution: LRI, CNRS UMR 8623 - UniversitÃcopyright Paris Sud
+ *              91405 Orsay, France *)
+
+(* $Id: FSetAVL_prog.v 616 2007-08-08 12:28:10Z msozeau $ *)
+
+Set Implicit Arguments.
+Unset Strict Implicit.
+
+Require Export Coq.Program.FunctionalExtensionality.
+
+Definition compose `A B C` (g : B -> C) (f : A -> B) := fun x : A => g (f x).
+
+Definition arrow (A B : Type) := A -> B.
+
+Definition impl (A B : Prop) : Prop := A -> B.
+
+Definition id `A` := fun x : A => x.
+
+Hint Unfold compose.
+
+Notation " g 'o' f " := (compose g f)  (at level 50, left associativity) : program_scope.
+
+Open Scope program_scope.
+
+Lemma compose_id_left : forall A B (f : A -> B), id o f = f.
+Proof.
+  intros.
+  unfold id, compose.
+  symmetry ; apply eta_expansion.
+Qed.
+
+Lemma compose_id_right : forall A B (f : A -> B), f o id = f.
+Proof.
+  intros.
+  unfold id, compose.
+  symmetry ; apply eta_expansion.
+Qed.
+
+Lemma compose_assoc : forall A B C D (f : A -> B) (g : B -> C) (h : C -> D), 
+  h o (g o f) = h o g o f.
+Proof.
+  reflexivity.
+Qed.
+
+Hint Rewrite @compose_id_left @compose_id_right @compose_assoc : core.
+
+Notation " f '#' x " := (f x) (at level 100, x at level 200, only parsing).
+
+Definition const `A B` (a : A) := fun x : B => a.
+
+Definition flip `A B C` (f : A -> B -> C) x y := f y x.
+
+Lemma flip_flip : forall A B C (f : A -> B -> C), flip (flip f) = f.
+Proof.
+  unfold flip.
+  intros.
+  extensionality x ; extensionality y.
+  reflexivity.
+Qed.
+
+Definition apply `A B` (f : A -> B) (x : A) := f x.
+
+(** Notations for the unit type and value. *)
+
+Notation " () " := Datatypes.unit : type_scope.
+Notation " () " := tt.
+
+(** Set maximally inserted implicit arguments for standard definitions. *)
+
+Implicit Arguments eq [[A]].
+
+Implicit Arguments Some [[A]].
+Implicit Arguments None [[A]].
+
+Implicit Arguments inl [[A] [B]].
+Implicit Arguments inr [[A] [B]].
+
+Implicit Arguments left [[A] [B]].
+Implicit Arguments right [[A] [B]].
+
+(** Curryfication. *)
+
+Definition curry `a b c` (f : a -> b -> c) (p : prod a b) : c :=
+  let (x, y) := p in f x y.
+
+Definition uncurry `a b c` (f : prod a b -> c) (x : a) (y : b) : c :=
+  f (x, y).
+
+Lemma uncurry_curry : forall a b c (f : a -> b -> c), uncurry (curry f) = f.
+Proof.
+  simpl ; intros.
+  unfold uncurry, curry.
+  extensionality x ; extensionality y.
+  reflexivity.
+Qed.
+
+Lemma curry_uncurry : forall a b c (f : prod a b -> c), curry (uncurry f) = f.
+Proof.
+  simpl ; intros.
+  unfold uncurry, curry.
+  extensionality x. 
+  destruct x ; simpl ; reflexivity.
+Qed.
+
+(** Useful implicits and notations for lists. *)
+
+Require Export Coq.Lists.List.
+
+Implicit Arguments nil [[A]].
+Implicit Arguments cons [[A]].
+
+Notation " [] " := nil.
+Notation " [ x ] " := (cons x nil).
+Notation " [ x ; .. ; y ] " := (cons x .. (cons y nil) ..).
+
+(** n-ary exists ! *)
+
+Notation "'exists' x y , p" := (ex (fun x => (ex (fun y => p))))
+  (at level 200, x ident, y ident, right associativity) : type_scope.
+
+Notation "'exists' x y z , p" := (ex (fun x => (ex (fun y => (ex (fun z => p))))))
+  (at level 200, x ident, y ident, z ident, right associativity) : type_scope.
+
+Notation "'exists' x y z w , p" := (ex (fun x => (ex (fun y => (ex (fun z => (ex (fun w => p))))))))
+  (at level 200, x ident, y ident, z ident, w ident, right associativity) : type_scope.
+
+Tactic Notation "exist" constr(x) := exists x.
+Tactic Notation "exist" constr(x) constr(y) := exists x ; exists y.
+Tactic Notation "exist" constr(x) constr(y) constr(z) := exists x ; exists y ; exists z.
+Tactic Notation "exist" constr(x) constr(y) constr(z) constr(w) := exists x ; exists y ; exists z ; exists w.
+
+Notation " ! A " := (notT A) (at level 200, A at level 100) : type_scope.
