theories/Program/Program.v
@@ -2,3 +2,4 @@ Require Export Coq.Program.Utils.
 Require Export Coq.Program.Wf.
 Require Export Coq.Program.Equality.
 Require Export Coq.Program.Subset.
+Require Export Coq.Program.Basics.
