tactics/class_setoid.ml4
@@ -42,22 +42,45 @@ let e_give_exact c gl =
 let assumption id = e_give_exact (mkVar id)
 
 let morphism_class = lazy (class_info (id_of_string "Morphism"))
-let morphism2_class = lazy (class_info (id_of_string "BinaryMorphism"))
-let morphism3_class = lazy (class_info (id_of_string "TernaryMorphism"))
 
 let get_respect cl = 
   Option.get (List.hd (Recordops.lookup_projections cl.cl_impl))
 
 let respect_proj = lazy (get_respect (Lazy.force morphism_class))
-let respect2_proj = lazy (get_respect (Lazy.force morphism2_class))
-let respect3_proj = lazy (get_respect (Lazy.force morphism3_class))
 
 let gen_constant dir s = Coqlib.gen_constant "Class_setoid" dir s
 let coq_proj1 = lazy(gen_constant ["Init"; "Logic"] "proj1")
 let coq_proj2 = lazy(gen_constant ["Init"; "Logic"] "proj2")
 let iff = lazy (gen_constant ["Init"; "Logic"] "iff")
+let impl = lazy (gen_constant ["Program"; "Basics"] "impl")
+let arrow = lazy (gen_constant ["Program"; "Basics"] "arrow")
+
+let reflexive_type = lazy (gen_constant ["Classes"; "Relations"] "Reflexive")
+let reflexive_proof = lazy (gen_constant ["Classes"; "Relations"] "reflexive")
+
+let symmetric_type = lazy (gen_constant ["Classes"; "Relations"] "Symmetric")
+let symmetric_proof = lazy (gen_constant ["Classes"; "Relations"] "symmetric")
+
+let transitive_type = lazy (gen_constant ["Classes"; "Relations"] "Transitive")
+let transitive_proof = lazy (gen_constant ["Classes"; "Relations"] "transitive")
+
+let inverse = lazy (gen_constant ["Classes"; "Relations"] "inverse")
+
+let respectful_dep = lazy (gen_constant ["Classes"; "Relations"] "respectful_dep")
+let respectful = lazy (gen_constant ["Classes"; "Relations"] "respectful")
+
+let iff_equiv = lazy (gen_constant ["Classes"; "Relations"] "iff_equivalence")
+let eq_equiv = lazy (gen_constant ["Classes"; "SetoidClass"] "eq_equivalence")
+
+(* let coq_relation = lazy (gen_constant ["Relations";"Relation_Definitions"] "relation") *)
+let coq_relation = lazy (gen_constant ["Classes";"Relations"] "relation")
+let coq_relationT = lazy (gen_constant ["Classes";"Relations"] "relationT")
+
+let setoid_refl_proj = lazy (gen_constant ["Classes"; "SetoidClass"] "equiv_refl")
 
 let iff_setoid = lazy (gen_constant ["Classes"; "SetoidClass"] "iff_setoid")
+let eq_setoid = lazy (gen_constant ["Classes"; "SetoidClass"] "eq_setoid")
+
 let setoid_equiv = lazy (gen_constant ["Classes"; "SetoidClass"] "equiv")
 let setoid_morphism = lazy (gen_constant ["Classes"; "SetoidClass"] "setoid_morphism")
 let setoid_refl_proj = lazy (gen_constant ["Classes"; "SetoidClass"] "equiv_refl")
@@ -70,12 +93,10 @@ let arrow_morphism a b =
 let setoid_refl pars x = 
   applistc (Lazy.force setoid_refl_proj) (pars @ [x])
       
-let class_one = lazy (Lazy.force morphism_class, Lazy.force respect_proj)
-let class_two = lazy (Lazy.force morphism2_class, Lazy.force respect2_proj)
-let class_three = lazy (Lazy.force morphism3_class, Lazy.force respect3_proj)
+let morphism_class = lazy (Lazy.force morphism_class, Lazy.force respect_proj)
 
-exception Found of (constr * constant * constr list * constr * constr array *
-		       (constr * (constr * constr * constr * constr * constr)) option array)
+exception Found of (constr * constr * (types * types) list * constr * constr array *
+		       (constr * (constr * constr * constr * constr)) option array)
 
 let resolve_morphism_evd env evd app = 
   let ev = Evarutil.e_new_evar evd env app in
@@ -88,79 +109,123 @@ let resolve_morphism_evd env evd app =
 let is_equiv env sigma t = 
   isConst t && Reductionops.is_conv env sigma (Lazy.force setoid_equiv) t
 
-let resolve_morphism env sigma direction oldt m args args' = 
-  let evars = ref (Evd.create_evar_defs Evd.empty) in
-  let morph_instance, proj, subst, m', args, args' = 
-    if is_equiv env sigma m then 
-      let params, rest = array_chop 3 args in
-      let a, r, s = params.(0), params.(1), params.(2) in
-      let params', rest' = array_chop 3 args' in
-      let inst = mkApp (Lazy.force setoid_morphism, params) in
-	(* Equiv gives a binary morphism *)
-      let (cl, proj) = Lazy.force class_two in
-      let ctxargs = [ a; r; s; a; r; s; mkProp; Lazy.force iff; Lazy.force iff_setoid; ] in
-      let m' = mkApp (m, [| a; r; s |]) in
-	inst, proj, ctxargs, m', rest, rest'
-    else
-      let cls =
+let split_head = function
+    hd :: tl -> hd, tl
+  | [] -> assert(false)
+
+let build_signature isevars env m cstrs finalcstr =
+  let new_evar isevars env t =
+    Evarutil.e_new_evar isevars env
+      (* ~src:(dummy_loc, ImplicitArg (ConstRef (Lazy.force respectful), (n, Some na))) *) t
+  in
+  let mk_relty ty obj =
+    let relty = mkApp (Lazy.force coq_relation, [| ty |]) in
+      match obj with
+	| None -> new_evar isevars env relty
+	| Some (p, (a, r, oldt, newt)) -> r
+  in
+  let rec aux t l =
+    let t = Reductionops.whd_betadelta env (Evd.evars_of !isevars) t in
+    match kind_of_term t, l with
+      | Prod (na, ty, b), obj :: cstrs -> 
+	  let (arg, evars) = aux b cstrs in
+	  let relty = mk_relty ty obj in
+	  let arg' = mkApp (Lazy.force respectful, [| ty ; relty ; b ; arg |]) in
+	    arg', (ty, relty) :: evars
+      | _, _ -> 
+	  (match finalcstr with
+	      None -> 
+		let rel = mk_relty t None in 
+		  rel, [t, rel]
+	    | Some (t, rel) -> rel, [t, rel])
+      | _, _ -> assert false
+  in aux m cstrs
+
+let reflexivity_proof env carrier relation x =
+  let goal = 
+    mkApp (Lazy.force reflexive_type, [| carrier ; relation |])
+  in
+    try let inst = resolve_one_typeclass env goal in
+	  mkApp (Lazy.force reflexive_proof, [| carrier ; relation ; inst ; x |])
+    with Not_found ->
+      let meta = Evarutil.new_meta() in
+	mkCast (mkMeta meta, DEFAULTcast, mkApp (relation, [| x; x |]))
+	  
+let resolve_morphism env sigma direction oldt m args args' cstr = 
+  let (morphism_cl, morphism_proj) = Lazy.force morphism_class in
+  let morph_instance, proj, sigargs, m', args, args' = 
+(*     if is_equiv env sigma m then  *)
+(*       let params, rest = array_chop 3 args in *)
+(*       let a, r, s = params.(0), params.(1), params.(2) in *)
+(*       let params', rest' = array_chop 3 args' in *)
+(*       let inst = mkApp (Lazy.force setoid_morphism, params) in *)
+(* 	(* Equiv gives a binary morphism *) *)
+(*       let (cl, proj) = Lazy.force class_two in *)
+(*       let ctxargs = [ a; r; s; a; r; s; mkProp; Lazy.force iff; Lazy.force iff_setoid; ] in *)
+(*       let m' = mkApp (m, [| a; r; s |]) in *)
+(* 	inst, proj, ctxargs, m', rest, rest' *)
+(*     else *)
+    let evars = ref (Evd.create_evar_defs Evd.empty) in
+    let pars =
 	match Array.length args with
-	    1 -> [Lazy.force class_one, 1]
-	  | 2 -> [Lazy.force class_two, 2; Lazy.force class_one, 1]
-	  | n -> [Lazy.force class_three, 3; Lazy.force class_two, 2; Lazy.force class_one, 1]
+	    1 -> [1]
+	  | 2 -> [2;1]
+	  | 3 -> [3;2;1]
+	  | _ -> [4;3;2;1]
       in
 	try 
-	  List.iter (fun ((cl, proj), n) ->
+	  List.iter (fun n ->
 	    evars := Evd.create_evar_defs Evd.empty;
-	    let cl_param, cl_context = match cl.cl_context with hd :: tl -> hd, tl | [] -> assert false in
-	    let ctxevs = substitution_of_named_context evars env cl.cl_name 0 [] (List.map snd cl_context) in
 	    let morphargs, morphobjs = array_chop (Array.length args - n) args in
 	    let morphargs', morphobjs' = array_chop (Array.length args - n) args' in
-	    let args = List.rev_map (fun (_, c) -> c) ctxevs in
 	    let appm = mkApp(m, morphargs) in
 	    let appmtype = Typing.type_of env sigma appm in
-	    let app = applistc (mkInd cl.cl_impl) (args @ [appm]) in
-	    let mtype = replace_vars ctxevs (pi3 (snd cl_param)) in
+	    let signature, sigargs = build_signature evars env appmtype (Array.to_list morphobjs') cstr in
+	    let cl_args = [| appmtype ; signature ; appm |] in
+	    let app = mkApp (mkInd morphism_cl.cl_impl, cl_args) in
 	      try 
-		evars := Evarconv.the_conv_x env appmtype mtype !evars;
-		evars := Evarutil.nf_evar_defs !evars;
-		let app = Evarutil.nf_isevar !evars app in
-		  raise (Found (resolve_morphism_evd env evars app, proj, args, appm, morphobjs, morphobjs'))
+		let morph = resolve_morphism_evd env evars app in
+		let evm = Evd.evars_of !evars in
+		let sigargs = List.map 
+		  (fun x, y -> Reductionops.nf_evar evm x, Reductionops.nf_evar evm y) 
+		  sigargs 
+		in
+		let appm = Reductionops.nf_evar evm appm in
+		let cl_args = Array.map (Reductionops.nf_evar evm) cl_args in
+		let proj = 
+		  mkApp (mkConst morphism_proj, 
+			Array.append cl_args [|morph|])
+		in
+		  raise (Found (morph, proj, sigargs, appm, morphobjs, morphobjs'))
 	      with Not_found -> ()
 		| Reduction.NotConvertible -> ()
 		| Stdpp.Exc_located (_, Pretype_errors.PretypeError _) 
 		| Pretype_errors.PretypeError _ -> ())
-	    cls; 
+	    pars;
 	  raise Not_found
 	with Found x -> x
   in 
-  evars := Evarutil.nf_evar_defs !evars;
-  let evm = Evd.evars_of !evars in
-  let ctxargs = List.map (Reductionops.nf_evar evm) subst in
-  let m' = Reductionops.nf_evar evm m' in
-  let appproj = applistc (mkConst proj) (ctxargs @ [m' ; morph_instance]) in
   let projargs, respars, typeargs = 
     array_fold_left2 
-      (fun (acc, ctxargs, typeargs') x y -> 
-	let par, ctx = list_chop 3 ctxargs in
+      (fun (acc, sigargs, typeargs') x y -> 
+	let (carrier, relation), sigargs = split_head sigargs in
 	  match y with
 	      None ->
-		let refl_proof = setoid_refl par x in
-		  [ refl_proof ; x ; x ] @ acc, ctx, x :: typeargs'
-	    | Some (p, (_, _, _, _, t')) ->
-		if direction then
-		  [ p ; t'; x ] @ acc, ctx, t' :: typeargs'
-		else [ p ; x; t' ] @ acc, ctx, t' :: typeargs')
-      ([], ctxargs, []) args args'
+		let refl_proof = reflexivity_proof env carrier relation x in
+		  [ refl_proof ; x ; x ] @ acc, sigargs, x :: typeargs'
+	    | Some (p, (_, _, _, t')) ->
+		[ p ; t'; x ] @ acc, sigargs, t' :: typeargs')
+      ([], sigargs, []) args args'
   in
-  let proof = applistc appproj (List.rev projargs) in
+  let proof = applistc proj (List.rev projargs) in
   let newt = applistc m' (List.rev typeargs) in
     match respars with
-	[ a ; r ; s ] -> (proof, (a, r, s, oldt, newt))
+	[ a, r ] -> (proof, (a, r, oldt, newt))
       | _ -> assert(false)
-      
-let build_new gl env setoid direction occs origt newt hyp hypinfo concl =
+
+let build_new gl env sigma direction occs origt newt hyp hypinfo concl cstr =
   let is_occ occ = occs = [] || List.mem occ occs in
-  let rec aux t occ = 
+  let rec aux t occ cstr =
     match kind_of_term t with
       | _ when eq_constr t origt -> 
 	  if is_occ occ then
@@ -170,70 +235,82 @@ let build_new gl env setoid direction occs origt newt hyp hypinfo concl =
       | App (m, args) ->
 	  let args', occ = 
 	    Array.fold_left 
-	      (fun (acc, occ) arg -> let res, occ = aux arg occ in (res :: acc, occ))
+	      (fun (acc, occ) arg -> let res, occ = aux arg occ None in (res :: acc, occ))
 	      ([], occ) args
 	  in
-	  let res = 
+	  let res =
 	    if List.for_all (fun x -> x = None) args' then None
 	    else 
 	      let args' = Array.of_list (List.rev args') in
-		(try Some (resolve_morphism env (project gl) direction t m args args')
+		(try Some (resolve_morphism env sigma direction t m args args' cstr)
 		  with Not_found -> None)
 	  in res, occ
 
       | Prod (_, x, b) -> 
-	  let x', occ = aux x occ in
-	  let b', occ = aux b occ in
+	  let x', occ = aux x occ None in
+	  let b', occ = aux b occ None in
 	  let res = 
 	    if x' = None && b' = None then None
 	    else 
-	      (try Some (resolve_morphism env (project gl) direction t (arrow_morphism (pf_type_of gl x) (pf_type_of gl b)) [| x ; b |] [| x' ; b' |])
+	      (try Some (resolve_morphism env sigma direction t
+			    (arrow_morphism (pf_type_of gl x) (pf_type_of gl b)) [| x ; b |] [| x' ; b' |]
+			    cstr)
 		with Not_found -> None)
 	  in res, occ
 
       | _ -> None, occ
-  in aux concl 1
+  in aux concl 1 cstr
 
-let decompose_setoid_eqhyp env sigma c dir t = 
-  match kind_of_term t with
-    | App (equiv, [| a; r; s; x; y |]) ->
-	if dir then (c, (a, r, s, x, y))
-	else (c, (a, r, s, y, x))
-    | App (r, args) when Array.length args >= 2 -> 
-	(try 
-	    let (p, (a, r, s, _, _)) = resolve_morphism env sigma dir t r args (Array.map (fun _ -> None) args) in
-	    let _, args = array_chop (Array.length args - 2) args in
-	      if dir then (c, (a, r, s, args.(0), args.(1)))
-	      else (c, (a, r, s, args.(1), args.(0)))
-	  with Not_found -> error "Not a (declared) setoid equality")
-    | _ -> error "Not a setoid equality"
+let decompose_setoid_eqhyp gl env sigma c left2right t = 
+  let (c, (car, rel, x, y) as res) =
+    match kind_of_term t with
+	(*     | App (equiv, [| a; r; s; x; y |]) -> *)
+	(* 	if dir then (c, (a, r, s, x, y)) *)
+	(* 	else (c, (a, r, s, y, x)) *)
+      | App (r, args) when Array.length args >= 2 -> 
+	  let relargs, args = array_chop (Array.length args - 2) args in
+	  let rel = mkApp (r, relargs) in
+	  let typ = pf_type_of gl rel in
+	    (match kind_of_term typ with
+	      | App (relation, [| carrier |]) when eq_constr relation (Lazy.force coq_relation) 
+		    || eq_constr relation (Lazy.force coq_relationT) ->
+		  (c, (carrier, rel, args.(0), args.(1)))
+	      | _ when isArity typ ->
+		  let (ctx, ar) = destArity typ in
+		    (match ctx with
+			[ (_, None, sx) ; (_, None, sy) ] when eq_constr sx sy -> 
+			  (c, (sx, rel, args.(0), args.(1)))
+		      | _ -> error "Only binary relations are supported")
+	      | _ -> error "Not a relation")
+      | _ -> error "Not a relation"
+  in
+    if left2right then res
+    else (c, (car, mkApp (Lazy.force inverse, [| car ; rel |]), y, x))
 
 let cl_rewrite_clause c left2right occs clause gl =
   let env = pf_env gl in
   let sigma = project gl in
   let hyp = pf_type_of gl c in
-  let hypt, (typ, rel, setoid, origt, newt as hypinfo) = decompose_setoid_eqhyp env sigma c left2right hyp in
+  let hypt, (typ, rel, origt, newt as hypinfo) = decompose_setoid_eqhyp gl env sigma c left2right hyp in
   let concl, is_hyp = 
     match clause with
 	Some ((_, id), _) -> pf_get_hyp_typ gl id, Some id
       | None -> pf_concl gl, None
   in
-  let eq, _ = build_new gl env setoid left2right occs origt newt hypt hypinfo concl in
+  let cstr = 
+    match is_hyp with
+	None -> (mkProp, mkApp (Lazy.force inverse, [| mkProp; Lazy.force impl |]))
+      | Some _ -> (mkProp, Lazy.force impl)
+  in
+  let eq, _ = build_new gl env sigma left2right occs origt newt hypt hypinfo concl (Some cstr) in
     match eq with  
-	Some (p, (_, _, _, _, t)) -> 
-	  let proj = 
-	    if left2right then 
-	      let proj = if is_hyp <> None then coq_proj1 else coq_proj2 in
-		applistc (Lazy.force proj)
-		  [ mkProd (Anonymous, concl, t) ; mkProd (Anonymous, t, concl) ; p ] 
-	    else 
-	      let proj = if is_hyp <> None then coq_proj2 else coq_proj1 in
-		applistc (Lazy.force proj)
-		  [ mkProd (Anonymous, t, concl) ; mkProd (Anonymous, concl, t) ; p ] 
-	  in
-	    (match is_hyp with
-	      | Some id -> Tactics.apply_in true id [proj,NoBindings]
-	      | None -> Tactics.apply proj) gl
+	Some (p, (_, _, oldt, newt)) -> 
+	  (match is_hyp with
+	    | Some id -> Tactics.apply_in true id [p,NoBindings]
+	    | None -> 
+		let meta = Evarutil.new_meta() in
+		let term = mkApp (p, [| mkCast (mkMeta meta, DEFAULTcast, newt) |]) in
+		  refine term) gl
       | None -> tclIDTAC gl
 	  
 open Extraargs
@@ -258,3 +335,17 @@ let clsubstitute o c =
 TACTIC EXTEND map_tac
 | [ "clsubstitute" orient(o) constr(c) ] -> [ clsubstitute o c ]
 END
+
+
+(* 
+	  let proj = 
+	    if left2right then 
+	      let proj = if is_hyp <> None then coq_proj1 else coq_proj2 in
+		applistc (Lazy.force proj)
+		  [ mkProd (Anonymous, concl, t) ; mkProd (Anonymous, t, concl) ; p ] 
+	    else 
+	      let proj = if is_hyp <> None then coq_proj2 else coq_proj1 in
+		applistc (Lazy.force proj)
+		  [ mkProd (Anonymous, t, concl) ; mkProd (Anonymous, concl, t) ; p ] 
+	  in
+*)
